code/experimental/P256/Hacl.Impl.ECDSA.MontgomeryMultiplication.fsti
@@ -38,13 +38,13 @@ let order_buffer: x: ilbuffer uint8 32ul {witnessed x prime_p256_order_seq /\ re
   createL_global prime_p256_order_list 
 
 
-val reduction_prime_prime_2prime_with_carry : x: widefelem -> result: felem ->
+val reduction_prime_2prime_with_carry : x: widefelem -> result: felem ->
   Stack unit 
     (requires fun h -> live h x /\ live h result /\  eq_or_disjoint x result /\ wide_as_nat h x < 2 * prime_p256_order)
     (ensures fun h0 _ h1 -> modifies (loc result) h0 h1 /\ as_nat h1 result = wide_as_nat h0 x % prime_p256_order)  
     
 
-val reduction_prime_prime_2prime_with_carry2 : carry: uint64 ->  x: felem -> result: felem ->
+val reduction_prime_2prime_with_carry2 : carry: uint64 ->  x: felem -> result: felem ->
   Stack unit 
     (requires fun h -> live h x /\ live h result /\ eq_or_disjoint x result /\ 
       uint_v carry * pow2 256 + as_nat h x < 2 * prime_p256_order )
